Adjust

src/BubbleSort.v
@@ -2,17 +2,265 @@ Require Import List Orders.
 Require Import Coq.Structures.OrdersFacts.
 Require Import Coq.Sorting.Permutation.
 Require Import Coq.Sorting.Sorted.
+Require Import Coq.Structures.GenericMinMax.
 Require Import Sorticoq.SortedList.
-Require Import Sorticoq.InsertionSort.
 Import ListNotations.
 
 Module BubbleSort (Import O: UsualOrderedTypeFull').
 
 Include (OrderedTypeFacts O).
 
+Module MinMax := GenericMinMax O.
+Import MinMax.
+
+Module Props := (UsualMinMaxProperties O MinMax).
+Import Props.
+
 Definition A := O.t.
 
+Definition max_of_list_t (l: list A) x : A :=
+  @fold_right A A max x l.
 
+Lemma max_of_list_t_ge_def: forall l x,
+  x <= max_of_list_t l x.
+Proof.
+  intros; induction l; simpl in *; intros.
+  - apply le_lteq. order.
+  - rewrite max_le_iff; intuition.
+Qed.
 
+Hint Resolve perm_skip perm_swap.
+Hint Constructors LocallySorted.
+Hint Extern 1 (?x <= ?y) => apply le_lteq; OrderTac.order.
+
+Lemma max_of_list_t_ok: forall l x,
+  forall x', In x' l -> x' <= max_of_list_t l x.
+Proof.
+  intros. induction l.
+  - inversion H.
+  - simpl. rewrite max_le_iff.
+    destruct H; subst; auto.
+Qed.
+
+Fixpoint bubble_step (l: list A) x : list A :=
+  match l with
+  | nil => [x]
+  | h::t => match O.compare x h with
+    | Gt => h::(bubble_step t x)
+    | _ => x::(bubble_step t h)
+    end
+  end.
+
+Lemma bubble_step_not_nil: forall l x,
+  bubble_step l x <> [].
+Proof.
+  intros l x H.
+  destruct l; simpl in *. inversion H.
+  destruct (compare x a); inversion H.
+Qed.
+
+Lemma last_l: forall (l: list A) x a,
+  l <> [] -> last (a::l) x = last l x.
+Proof.
+  induction l; intuition.
+Qed.
+
+Lemma max_niv: forall l x,
+  max x (max_of_list_t l x) = max_of_list_t l x.
+Proof.
+  intros. induction l; simpl.
+  - apply max_id.
+  - rewrite max_assoc; rewrite (max_comm x a).
+    rewrite <- max_assoc; change (gmax compare) with max.
+    rewrite IHl. reflexivity.
+Qed.
+
+Lemma max_rev: forall l x a,
+  max x (max_of_list_t l a) = max a (max_of_list_t l x).
+Proof.
+  intros. induction l; simpl.
+  - apply max_comm.
+  - do 2 rewrite max_assoc. rewrite (max_comm x a0).
+    rewrite (max_comm a a0). do 2 rewrite <- max_assoc.
+    change (gmax compare) with max.
+    rewrite IHl. reflexivity.
+Qed.
+
+Lemma max_lt: forall l x a,
+  a < x ->
+  max x (max_of_list_t l a) = max_of_list_t l x.
+Proof.
+  intros. induction l; simpl.
+  - apply max_l. apply le_lteq. auto.
+  - rewrite max_assoc. rewrite (max_comm x a0).
+    rewrite <- max_assoc. change (gmax compare) with max.
+    rewrite IHl. reflexivity.
+Qed.
+
+Ltac convert_compare :=
+  repeat match goal with
+  | H: compare ?x ?y = Lt |- _ => apply compare_lt_iff in H
+  | H: compare ?x ?y = Gt |- _ => apply compare_gt_iff in H
+  | H: compare ?x ?y = Eq |- _ => apply compare_eq in H
+  end.
+
+Ltac do_compare :=
+  let C := fresh in let eqnC := fresh in remember (compare _ _) as C eqn:eqnC;
+  symmetry in eqnC; destruct C; convert_compare.
+
+Lemma bubble_step_bubbles: forall l x x',
+  last (bubble_step l x) x' = max_of_list_t l x.
+Proof.
+  induction l; intuition.
+  simpl (max_of_list_t _ _).
+  assert (forall x, bubble_step l x <> []) by apply bubble_step_not_nil.
+  simpl; do_compare.
+  all: match goal with
+  | |- last (?a :: bubble_step _ ?x) _ = _ =>
+    specialize H with x; apply (last_l _ x' a) in H; rewrite H; rewrite IHl;
+    symmetry; subst
+  end.
+  - apply max_niv.
+  - apply max_lt; auto.
+  - rewrite max_rev; apply max_lt; auto.
+Qed.
+
+Lemma bubble_step_length: forall l a,
+  length (bubble_step l a) = length (a::l).
+Proof.
+  induction l; intros. intuition.
+  simpl; do_compare; simpl; rewrite IHl; auto.
+Qed.
+
+Lemma bubble_step_permute: forall l a,
+  Permutation (a::l) (bubble_step l a).
+Proof.
+  induction l; intros; auto.
+  simpl. do_compare; auto.
+  transitivity (a::a0::l); auto.
+Qed.
+
+Require Import Omega.
+
+Fixpoint bubble_sort_m (l: list A) (m: nat) : list A :=
+  match l, m with
+  | nil, _ => nil
+  | _, 0 => nil
+  | h::t, S m' => let l' := (bubble_step t h) in
+    (bubble_sort_m (removelast l') m') ++ [last l' h]
+  end.
+
+Definition bubble_sort (l: list A) :=
+  bubble_sort_m l (length l).
+
+Ltac stupid_list :=
+  intro Y; inversion Y.
+
+Lemma removelast_end: forall (l: list A) x,
+  removelast (l ++ [x]) = l.
+Proof.
+  intros. rewrite removelast_app. ssimpl_list. reflexivity.
+  stupid_list.
+Qed.
+
+Lemma permute_omg: forall (l: list A) a,
+  Permutation (l) (removelast (l ++ [a])).
+Proof.
+  intros; rewrite removelast_end; auto.
+Qed.
+
+Lemma removelast_len: forall l a,
+  length (removelast (bubble_step l a)) = length l.
+Proof.
+  intros.
+  assert (bubble_step l a <> []) by apply bubble_step_not_nil.
+  apply exists_last in H. inversion H; inversion X. rewrite H0.
+  rewrite removelast_end. apply f_equal with (f:=@length A) in H0.
+  rewrite bubble_step_length in H0. rewrite app_length in H0; simpl in H0.
+  intuition.
+Qed.
+
+Lemma permute: forall n l,
+  length l = n -> Permutation l (bubble_sort l).
+Proof.
+  induction n; intros.
+  - apply length_zero_iff_nil in H; subst; auto.
+  - destruct l; simpl; auto.
+    unfold bubble_sort in *. simpl.
+    specialize IHn with (removelast (bubble_step l a)).
+    rewrite removelast_len in IHn. simpl in H. apply eq_add_S in H.
+    apply IHn in H.
+    transitivity (removelast (bubble_step l a) ++ [last (bubble_step l a) a]).
+    + assert (bubble_step l a <> []) by apply bubble_step_not_nil.
+      apply app_removelast_last with (d:=a) in H0. rewrite <- H0.
+      apply bubble_step_permute.
+    + apply Permutation_app_tail. assumption.
+Qed.
+
+Corollary bubble_sort_permute: forall l,
+  Permutation l (bubble_sort l).
+Proof.
+  intros; apply (permute (length l) _); reflexivity.
+Qed.
+
+Lemma bubble_sort_not_nil: forall l,
+  l <> [] -> bubble_sort l <> [].
+Proof.
+  intros. destruct l; try contradiction.
+  unfold bubble_sort; simpl. intro Y.
+  apply app_eq_nil in Y. destruct Y. inversion H1.
+Qed.
+
+Include (OTF_to_TTLB O).
+Lemma le_trans:
+  Transitive le.
+Proof.
+  unfold Transitive. intros. rewrite <- leb_le in *.
+  unfold is_true in *. unfold leb in *; repeat do_compare; subst; auto; order.
+Qed.
+
+Hint Resolve le_trans.
+
+Lemma In_removelast: forall {A:Type} l x,
+  @In A x (removelast l) -> In x l.
+Proof.
+  intros. destruct l; auto.
+  assert (a::l <> []) by stupid_list.
+  apply app_removelast_last with (d:=a) in H0. rewrite H0.
+  apply in_or_app; auto.
+Qed.
+
+Lemma BubbleSortHelp_is_LocallySorted: forall l n,
+  length l = n ->
+    LocallySorted le (bubble_sort_m l n).
+Proof.
+  intros; generalize dependent l;
+  induction n; intros.
+  - apply length_zero_iff_nil in H. subst; simpl. auto.
+  - destruct l; simpl in *. inversion H.
+    assert (length (removelast (bubble_step l a)) = n).
+      transitivity (length l).
+      apply removelast_len. auto.
+    apply LocallySorted_end_relation; auto.
+    intros. rewrite <- H0 in H1.
+    change (bubble_sort_m ?x (length ?x)) with (bubble_sort x) in H1.
+    rewrite bubble_step_bubbles.
+    assert (Permutation (bubble_sort (removelast (bubble_step l a))) (removelast (bubble_step l a))).
+      apply Permutation_sym; apply bubble_sort_permute.
+    apply Permutation_in with (x:=t0)in H2; auto.
+    apply In_removelast in H2.
+    assert (Permutation (bubble_step l a) (a::l)).
+      apply Permutation_sym; apply bubble_step_permute.
+    apply Permutation_in with (x:=t0) in H3; auto.
+    destruct H3; subst.
+    apply max_of_list_t_ge_def.
+    apply max_of_list_t_ok; auto.
+Qed.
+
+Lemma BubbleSort_LocallySorted: forall l,
+  LocallySorted le (bubble_sort l).
+Proof.
+  intros. apply BubbleSortHelp_is_LocallySorted. auto.
+Qed.
 
 End BubbleSort.
